Restructureing

theories/Analysis/AnalysisForwardSSA.v
@@ -1,63 +1,60 @@
 Require Import CSet Le ListUpdateAt Coq.Classes.RelationClasses.
 
 Require Import Plus Util AllInRel Map Terminating MoreInversion.
-Require Import Val Var Env IL Annotation Infra.Lattice.
+Require Import Val Var Env IL Annotation Infra.Lattice AnnotationLattice.
 Require Import DecSolve LengthEq MoreList Status AllInRel OptionR.
-Require Import Keep Subterm Analysis CMapPartialOrder DomainSSA.
+Require Import Keep Subterm Analysis CMapPartialOrder DomainSSA CMapTerminating.
 
 Set Implicit Arguments.
 
-
-Definition joinTopAnn A `{JoinSemiLattice A} (a:ann A) (b:A) :=
-  setTopAnn a (join (getAnn a) b).
-
-Definition forwardF (D:Type) (BL:list bool)
-           (forward: forall (s:stmt) (d:Dom D) (anr:ann bool),  Dom D * ann bool * list bool)
-           (F:list (params * stmt)) (rF:list (ann bool)) (a:Dom D)
-  : Dom D * list (ann bool) * list bool.
-  revert F rF a.
+Definition forwardF (sT:stmt) (Dom:stmt->Type) (BL:list bool)
+           (forward: forall s (ST:subTerm s sT) (d:Dom sT) (anr:ann bool), Dom sT * ann bool * list bool)
+           (F:list (params * stmt)) (rF:list (ann bool)) (a:Dom sT)
+           (ST:forall n s, get F n s -> subTerm (snd s) sT)
+  : Dom sT * list (ann bool) * list bool.
+  revert F rF ST a.
   fix g 1. intros.
   destruct F as [|Zs F'].
   - eapply (a, nil, BL).
   - destruct rF as [|b rF'].
     + eapply (a, nil, BL).
-    + pose (p:=forward (snd Zs) a b).
-      pose (q:=g F' rF' (fst (fst p))).
+    + pose (p:=forward (snd Zs) ltac:(eauto using get) a b).
+      pose (q:=g F' rF' ltac:(eauto using get) (fst (fst p))).
       eapply (fst (fst q),
               snd (fst p) :: (snd (fst q)),
               zip join (snd p) (snd q)).
 Defined.
 
-Arguments forwardF [D] BL forward F rF a.
+Arguments forwardF [sT] [Dom] BL forward F rF a ST.
 
-Fixpoint forwardF_length (D:Type) BL forward
+Fixpoint forwardF_length (sT:stmt) (Dom:stmt->Type) BL forward
            (F:list (params * stmt)) rF a
-           {struct F}
-  : length (snd (fst (@forwardF D BL forward F rF a))) = min (length F) (length rF).
+           (ST:forall n s, get F n s -> subTerm (snd s) sT) {struct F}
+  : length (snd (fst (@forwardF sT Dom BL forward F rF a ST))) = min (length F) (length rF).
 Proof.
   destruct F as [|Zs F'], rF; simpl; eauto.
 Qed.
 
-Lemma forwardF_snd_length (D:Type) BL
-      (forward: forall (s:stmt) (d:Dom D) (anr:ann bool), Dom D * ann bool * list bool)
+Lemma forwardF_snd_length (sT:stmt) (Dom:stmt->Type) BL
+      (forward: forall s (ST:subTerm s sT) (d:Dom sT) (anr:ann bool), Dom sT * ann bool * list bool)
       (F:list (params * stmt)) rF a
-      k
-      (LEN:forall n Zs d r, get F n Zs -> length (snd (@forward (snd Zs) d r)) = k)
+      (ST:forall n Zs, get F n Zs -> subTerm (snd Zs) sT) k
+      (LEN:forall n Zs ST d r, get F n Zs -> length (snd (@forward (snd Zs) ST d r)) = k)
       (LenBL: length BL = k)
-  : length (snd (@forwardF D BL forward F rF a)) = k.
+  : length (snd (@forwardF sT Dom BL forward F rF a ST)) = k.
 Proof.
   general induction F; destruct rF; simpl; eauto.
   len_simpl. erewrite IHF; eauto using get.
   erewrite LEN; eauto using get with len.
 Qed.
 
-Lemma forwardF_snd_length' (D:Type) BL
-      (forward: forall (s:stmt) (d:Dom D) (anr:ann bool), Dom D * ann bool * list bool)
+Lemma forwardF_snd_length' (sT:stmt) (Dom:stmt->Type) BL
+      (forward: forall s (ST:subTerm s sT) (d:Dom sT) (anr:ann bool), Dom sT * ann bool * list bool)
       (F:list (params * stmt)) rF a
-      k
-      (LEN:forall n Zs d r, get F n Zs -> length (snd (@forward (snd Zs) d r)) = k)
+      (ST:forall n Zs, get F n Zs -> subTerm (snd Zs) sT) k
+      (LEN:forall n Zs ST d r, get F n Zs -> length (snd (@forward (snd Zs) ST d r)) = k)
       (Leq: k <= length BL) (LenF:❬F❭ > 0) (LenrF:❬rF❭ > 0)
-  : length (snd (@forwardF D BL forward F rF a)) = k.
+  : length (snd (@forwardF sT Dom BL forward F rF a ST)) = k.
 Proof.
   general induction F; destruct rF; simpl in *; eauto; try omega.
   len_simpl.
@@ -66,17 +63,16 @@ Proof.
   erewrite LEN; eauto using get with len.
 Qed.
 
-
 Smpl Add
      match goal with
-     | [ |- context [ ❬snd (fst (@forwardF ?D ?BL ?f ?F ?rF ?a))❭ ] ] =>
-       rewrite (@forwardF_length D BL f F rF a)
-     | [ H : context [ ❬snd (fst (@forwardF ?D ?BL ?f ?F ?rF ?a))❭ ] |- _ ] =>
-       rewrite (@forwardF_length D BL f F rF a) in H
-     | [ |- context [ ❬snd (@forwardF ?D ?BL ?f ?F ?rF ?a)❭ ] ] =>
-       erewrite (@forwardF_snd_length D BL f F rF a)
-     | [ H : context [ ❬snd (@forwardF ?D ?BL ?f ?F ?rF ?a)❭ ] |- _ ] =>
-       erewrite (@forwardF_snd_length D BL f F rF a) in H
+     | [ |- context [ ❬snd (fst (@forwardF ?sT ?Dom ?BL ?f ?F ?rF ?a ?ST))❭ ] ] =>
+       rewrite (@forwardF_length sT Dom BL f F rF a ST)
+     | [ H : context [ ❬snd (fst (@forwardF ?sT ?Dom ?BL ?f ?F ?rF ?a ?ST))❭ ] |- _ ] =>
+       rewrite (@forwardF_length sT Dom BL f F rF a ST) in H
+     | [ |- context [ ❬snd (@forwardF ?sT ?Dom ?BL ?f ?F ?rF ?a ?ST)❭ ] ] =>
+       erewrite (@forwardF_snd_length sT Dom BL f F rF a ST)
+     | [ H : context [ ❬snd (@forwardF ?sT ?Dom ?BL ?f ?F ?rF ?a ?ST)❭ ] |- _ ] =>
+       erewrite (@forwardF_snd_length sT Dom BL f F rF a ST) in H
      end : len.
 
 Lemma ZLIncl_ext sT st F t (ZL:list params)
@@ -94,60 +90,69 @@ Proof.
   cset_tac.
 Qed.
 
-Lemma subTerm_EQ_If_freeVars_e
-  : forall (sT st : stmt) (e : op) (s t : stmt),
-    st = stmtIf e s t -> subTerm st sT -> Op.freeVars e ⊆ occurVars sT.
+Lemma ZLIncl_App_Z sT ZL n
+      (Incl:list_union (of_list ⊝ ZL) [<=] occurVars sT)
+  : of_list (nth n ZL (nil : params)) [<=] occurVars sT.
 Proof.
-  intros; subst.
-  eapply subTerm_occurVars in H0. simpl in *.
-  cset_tac.
+  destruct (get_dec ZL n); dcr.
+  - erewrite get_nth; eauto. rewrite <- Incl.
+    eapply incl_list_union; eauto using zip_get.
+  - rewrite not_get_nth_default; eauto.
+    simpl. cset_tac.
 Qed.
 
+Arguments ZLIncl_App_Z {sT} {ZL} n Incl.
 
+Definition sTDom D sT := VDom (occurVars sT) D.
 
-Fixpoint forward (D: Type) `{JoinSemiLattice D}
-           (exp_transf : bool -> Dom D -> exp -> option D)
-           (reach_transf : bool -> Dom D -> op -> bool * bool)
-           (ZL:list (params))
-           (st:stmt) (d:Dom D) (anr:ann bool) {struct st}
-  :  Dom D * ann bool * list bool.
+Fixpoint forward (sT:stmt) (D: Type) `{JoinSemiLattice D}
+         (exp_transf : forall U, bool -> VDom U D -> exp -> option D)
+         (reach_transf : forall U, bool -> VDom U D -> op -> bool * bool)
+         (ZL:list (params)) (ZLIncl:list_union (of_list ⊝ ZL) [<=] occurVars sT)
+         (st:stmt) (ST:subTerm st sT) (d:VDom (occurVars sT) D) (anr:ann bool) {struct st}
+  :  VDom (occurVars sT) D * ann bool * list bool.
   refine (
-      match st as st', anr return Dom D * ann bool * list bool with
+      match st as st', anr return st = st' -> VDom (occurVars sT) D * ann bool * list bool with
       | stmtLet x e s as st, ann1 b anr' =>
-          let d:Dom D := domupd d x (exp_transf b d e) in
+        fun EQ =>
+          let d:VDom (occurVars sT) D := domupdd d (exp_transf _ b d e) (subTerm_EQ_Let_x EQ ST) in
           let '(d', ans', AL) :=
-              forward D _ _ exp_transf reach_transf
-                      ZL s d (setTopAnn anr' b) in
+              forward sT D _ _ exp_transf reach_transf
+                      ZL ZLIncl s (subTerm_EQ_Let EQ ST) d (setTopAnn anr' b) in
           (d', ann1 b ans', AL)
       | stmtIf e s t, ann2 b anr1 anr2 =>
-          let '(b1,b2) := reach_transf b d e in
+        fun EQ =>
+          let '(b1,b2) := reach_transf _ b d e in
           let '(a', an1, AL1) :=
-              @forward D _ _ exp_transf reach_transf ZL s
-                       d (setTopAnn anr1 b1) in
+              @forward _ D _ _ exp_transf reach_transf ZL ZLIncl s
+                       (subTerm_EQ_If1 EQ ST) d (setTopAnn anr1 b1) in
           let '(a'', an2, AL2) :=
-              @forward D _ _ exp_transf reach_transf ZL t
-                       a' (setTopAnn anr2 b2) in
+              @forward _ D _ _ exp_transf reach_transf ZL ZLIncl t
+                       (subTerm_EQ_If2 EQ ST) a' (setTopAnn anr2 b2) in
           (a'', ann2 b an1 an2, zip join AL1 AL2)
       | stmtApp f Y as st, ann0 b =>
+        fun EQ =>
           let Z := nth (counted f) ZL (nil:list var) in
-          let Yc := List.map (Operation ∘ exp_transf b d) Y in
+          let Yc := List.map (Operation ∘ exp_transf _ b d) Y in
           (* we assume renamed apart here, so it's ok to leave definitions
        in d[X <-- Yc] that are /not/ defined at the point where f is defined *)
           let AL := ((fun _ => false) ⊝ ZL) in
-          (if b then domjoin_list d Z Yc else d, ann0 b, list_update_at AL (counted f) b)
-    | stmtReturn x as st, ann0 b =>
-      (d, ann0 b, ((fun _ => false) ⊝ ZL))
-
-    | stmtFun F t as st, annF b rF r =>
-        let ZL' := List.map fst F ++ ZL in
-        let '(a', r', AL) :=
-            @forward D _ _ exp_transf reach_transf ZL'
-                     t d (setTopAnn r b) in
-        let '(a'', rF', AL') := forwardF AL (forward D _ _ exp_transf reach_transf ZL')
-                            F (zip (@joinTopAnn _ _ _) rF AL) a' in
-        (a'', annF b (zip (@setTopAnn _) rF' AL') r', drop (length F) AL')
-    | _, _ => (d, anr, ((fun _ => false) ⊝ ZL))
-      end).
+          (if b then domjoin_listd d Z Yc (ZLIncl_App_Z (counted f) ZLIncl) else d, ann0 b, list_update_at AL (counted f) b)
+      | stmtReturn x as st, ann0 b =>
+        fun EQ =>
+          (d, ann0 b, ((fun _ => false) ⊝ ZL))
+      | stmtFun F t as st, annF b rF r =>
+        fun EQ =>
+          let ZL' := List.map fst F ++ ZL in
+          let '(a', r', AL) :=
+              @forward sT D _ _ exp_transf reach_transf ZL' (ZLIncl_ext ZL EQ ST ZLIncl)
+                       t (subTerm_EQ_Fun1 EQ ST) d (setTopAnn r b) in
+          let '(a'', rF', AL') := @forwardF sT (sTDom D) AL (forward sT D _ _ exp_transf reach_transf ZL' (ZLIncl_ext ZL EQ ST ZLIncl))
+                                          F (zip (@joinTopAnn _ _ _) rF AL)
+                                          a'(subTerm_EQ_Fun2 EQ ST)  in
+          (a'', annF b (zip (@setTopAnn _) rF' AL') r', drop (length F) AL')
+      | _, _ => fun _ => (d, anr, ((fun _ => false) ⊝ ZL))
+      end eq_refl).
 Defined.
 
 Smpl Add 100
@@ -159,90 +164,65 @@ Smpl Add 100
      end : len.
 
 
-Lemma forward_length D `{JoinSemiLattice D} f fr ZL s d r
-  : ❬snd (forward f fr ZL s d r)❭ = ❬ZL❭.
+Lemma forward_length (sT:stmt) D `{JoinSemiLattice D} f fr ZL ZLIncl s (ST:subTerm s sT) d r
+  : ❬snd (forward f fr ZL ZLIncl ST d r)❭ = ❬ZL❭.
 Proof.
   revert_except s.
   sind s; destruct s, r; simpl; eauto with len;
     repeat let_pair_case_eq; subst; simpl; eauto.
   - len_simpl. rewrite (IH s1), (IH s2); eauto with len.
   - rewrite length_drop_minus.
-    erewrite forwardF_snd_length; eauto with len.
-    + len_simpl. omega.
+    len_simpl; try reflexivity.
+    + rewrite IH; eauto. len_simpl. omega.
+    + intros. rewrite !IH; eauto.
 Qed.
 
-Lemma forward_fst_snd_getAnn D `{JoinSemiLattice D} f fr ZL s d r
-  : getAnn (snd (fst (forward f fr ZL s d r))) = getAnn r.
+Smpl Add 100
+     match goal with
+     | [ H : context [ ❬snd (@forward ?sT ?D ?PO ?JSL ?f ?fr ?ZL ?ZLIncl ?s ?ST ?d ?r)❭ ] |- _ ] =>
+       setoid_rewrite (@forward_length sT D PO JSL f fr ZL ZLIncl s ST d r) in H
+     | [ |- context [ ❬snd (@forward ?sT ?D ?PO ?JSL ?f ?fr ?ZL ?ZLIncl ?s ?ST ?d ?r)❭ ] ] =>
+       setoid_rewrite (@forward_length sT D PO JSL f fr ZL ZLIncl s ST d r)
+     end : len.
+
+Lemma forward_fst_snd_getAnn sT D `{JoinSemiLattice D} f fr ZL ZLIncl
+      s (ST:subTerm s sT) d r
+  : getAnn (snd (fst (forward f fr ZL ZLIncl ST d r))) = getAnn r.
 Proof.
   revert_except s.
   sind s; destruct s, r; simpl; eauto with len;
     repeat let_pair_case_eq; subst; simpl; eauto.
 Qed.
 
-Lemma forward_getAnn D `{JoinSemiLattice D} f fr ZL s b r r'
-  : ann_R poEq (snd (fst (forward f fr ZL s b r))) r'
+Lemma forward_getAnn sT D `{JoinSemiLattice D} f fr ZL ZLIncl s (ST:subTerm s sT) b r r'
+  : ann_R poEq (snd (fst (forward f fr ZL ZLIncl ST b r))) r'
     -> getAnn r = getAnn r'.
 Proof.
   intros. eapply ann_R_get in H1.
   rewrite forward_fst_snd_getAnn in H1. eauto.
 Qed.
 
-
-Lemma setTopAnn_eta' A (a:ann A)
-  : (setTopAnn a (getAnn a)) = a.
-Proof.
-  destruct a; simpl; eauto.
-Qed.
-
-Smpl Add 100
-     match goal with
-     | [ H : context [ ❬snd (@forward ?D ?PO ?JSL ?f ?fr ?ZL ?s ?d ?r)❭ ] |- _ ] =>
-       rewrite (@forward_length D PO JSL f fr ZL s d r) in H
-     | [ |- context [ ❬snd (@forward ?D ?PO ?JSL ?f ?fr ?ZL ?s ?d ?r)❭ ] ] =>
-       rewrite (@forward_length D PO JSL f fr ZL s d r)
-     end : len.
-
-Lemma forwardF_mon (D:Type) `{JoinSemiLattice D} f fr ZL BL (Len:❬BL❭ <= ❬ZL❭)
-      (F:list (params * stmt)) rF a
-  : PIR2 poLe BL (snd (@forwardF D BL (forward f fr ZL) F rF a)).
+Lemma forwardF_mon sT (D:Type) `{JoinSemiLattice D} f fr ZL ZLIncl BL
+      (Len:❬BL❭ <= ❬ZL❭)
+      (F:list (params * stmt)) STF rF a
+  : PIR2 poLe BL (snd (@forwardF sT (sTDom D) BL (forward f fr ZL ZLIncl) F rF a STF)).
 Proof.
   revert rF a.
   induction F; intros; destruct rF; simpl; eauto.
   eapply PIR2_impb_orb_left; eauto with len.
 Qed.
 
-Lemma forwardF_mon' (D:Type) `{JoinSemiLattice D} f fr ZL (F:list (params * stmt)) rF BL
+Lemma forwardF_mon' sT (D:Type) `{JoinSemiLattice D}
+      f fr ZL ZLIncl (F:list (params * stmt)) rF BL STF
        (Len:❬F❭ = ❬rF❭) a
   : PIR2 poEq (getAnn ⊝ rF)
-         (getAnn ⊝ snd (fst (forwardF BL
-                                      (forward f fr ZL) F rF a))).
+         (getAnn ⊝ snd (fst (@forwardF sT (sTDom D) BL
+                                       (forward f fr ZL ZLIncl) F rF a STF))).
 Proof.
   general induction Len; intros; simpl; eauto.
   econstructor.
-  - rewrite forward_fst_snd_getAnn. reflexivity.
+  - setoid_rewrite forward_fst_snd_getAnn. reflexivity.
   - eapply IHLen.
-Qed.
-
-Lemma fold_list_length A B (f:list B -> (list A * bool) -> list B) (a:list (list A * bool)) (b: list B)
-  : (forall n aa, get a n aa -> ❬b❭ <= ❬fst aa❭)
-    -> (forall aa b, ❬b❭ <= ❬fst aa❭ -> ❬f b aa❭ = ❬b❭)
-    -> length (fold_left f a b) = ❬b❭.
-Proof.
-  intros LEN.
-  general induction a; simpl; eauto.
-  erewrite IHa; eauto 10 using get with len.
-  intros. rewrite H; eauto using get.
-Qed.
-
-Lemma fold_list_length' A B (f:list B -> (list A) -> list B) (a:list (list A)) (b: list B)
-  : (forall n aa, get a n aa -> ❬b❭ <= ❬aa❭)
-    -> (forall aa b, ❬b❭ <= ❬aa❭ -> ❬f b aa❭ = ❬b❭)
-    -> length (fold_left f a b) = ❬b❭.
-Proof.
-  intros LEN.
-  general induction a; simpl; eauto.
-  erewrite IHa; eauto 10 using get with len.
-  intros. rewrite H; eauto using get.
 Qed.
 
 Ltac fold_po :=
@@ -255,54 +235,28 @@ Ltac fold_po :=
            change (ann_R poLe x y) with (poLe x y)
   end.
 
-Lemma fold_left_join_struct T `{JoinSemiLattice T} (A A':list T) (b b':T)
-  : PIR2 poLe A A'
-    -> b ⊑ b'
-    -> fold_left join A b ⊑ fold_left join A' b'.
-Proof.
-  intros pir.
-  general induction pir; simpl; eauto.
-  eapply IHpir.
-  eapply join_struct; eauto.
-Qed.
-
 Require Import FiniteFixpointIteration.
 
-Lemma option_map_mon T `{PartialOrder T}  U `{PartialOrder U} (a a':option T) (f f': T -> U)
-  : a ⊑ a'
-    -> (forall x y, x ⊑ y -> f x ⊑ f' y)
-    -> option_map f a ⊑ option_map f' a'.
-Proof.
-  intros A; inv A; simpl;
-    clear_trivial_eqs; simpl; eauto using fstNoneOrR.
-Qed.
-
-Lemma PIR2_bottom_least A B `{LowerBounded A} (ZL:list B) (l:list A)
-  : ❬ZL❭ = ❬l❭
-    -> PIR2 poLe (tab (⊥) ‖ZL‖) l.
-Proof.
-  intros. eapply PIR2_get; intros; inv_get; eauto with len.
-  eapply bottom_least.
-Qed.
-
-Lemma forwardF_monotone D `{JoinSemiLattice D}
-      (forward forward' : stmt -> Dom D -> ann bool -> Dom D * ann bool * 〔bool〕) F
-      (fwdMon:forall  n Zs (GET:get F n Zs),
-          forall (d d' : Dom D),
+Lemma forwardF_monotone (sT:stmt) (Dom : stmt -> Type) `{PartialOrder (Dom sT)}
+      (forward forward' : forall s : stmt,
+          subTerm s sT -> Dom sT -> ann bool -> Dom sT * ann bool * 〔bool〕) F
+      (fwdMon:forall  n Zs (GET:get F n Zs) (ST:subTerm (snd Zs) sT),
+          forall (d d' : Dom sT),
             d ⊑ d'
             -> forall (r r':ann bool),
               r ⊑ r'
-              -> forward (snd Zs) d r ⊑ forward' (snd Zs) d' r')
-  : forall (d d' : Dom D),
+              -> forward (snd Zs) ST d r ⊑ forward' (snd Zs) ST d' r')
+  : forall ST,
+    forall (d d' : Dom sT),
       d ⊑ d'
       -> forall (rF rF':list (ann bool)),
         rF ⊑ rF'
         -> forall (BL BL':list bool),
           BL ⊑ BL'
-        -> forwardF BL forward F rF d
-                   ⊑  forwardF BL' forward' F rF' d'.
+        -> forwardF BL forward F rF d ST
+                   ⊑  forwardF BL' forward' F rF' d' ST.
 Proof.
-  intros d d' LE_d rF rF' LE_rf.
+  intros ST d d' LE_d rF rF' LE_rf.
   general induction F; inv LE_rf; simpl;
     try now (econstructor; simpl; eauto using @ann_R, @PIR2).
   split; [split|].
@@ -316,33 +270,26 @@ Proof.
     eapply IHF; eauto using get. eapply fwdMon; eauto using get.
 Qed.
 
-Lemma PIR2_eq_zip X Y Z (f:X -> Y -> Z) l1 l2 l1' l2'
-  : PIR2 eq l1 l1'
-    -> PIR2 eq l2 l2'
-    -> PIR2 eq (zip f l1 l2) (zip f l1' l2').
-Proof.
-  intros P1 P2.
-  general induction P1; inv P2; simpl; econstructor; eauto.
-Qed.
-
-Lemma forwardF_ext D `{JoinSemiLattice D}
-      (forward forward' : stmt -> Dom D -> ann bool -> Dom D * ann bool * 〔bool〕) F
-      (fwdMon:forall  n Zs (GET:get F n Zs),
-          forall (d d' : Dom D),
+Lemma forwardF_ext (sT:stmt) (Dom : stmt -> Type) `{PartialOrder (Dom sT)}
+      (forward forward' : forall s : stmt,
+          subTerm s sT -> Dom sT -> ann bool -> Dom sT * ann bool * 〔bool〕) F
+      (fwdMon:forall  n Zs (GET:get F n Zs) (ST:subTerm (snd Zs) sT),
+          forall (d d' : Dom sT),
             poEq d d'
             -> forall (r r':ann bool),
               poEq r r'
-              -> poEq (forward (snd Zs) d r) (forward' (snd Zs) d' r'))
-  : forall (d d' : Dom D),
+              -> poEq (forward (snd Zs) ST d r) (forward' (snd Zs) ST d' r'))
+  : forall ST,
+    forall (d d' : Dom sT),
       poEq d d'
       -> forall (rF rF':list (ann bool)),
         poEq rF rF'
         -> forall (BL BL':list bool),
           poEq BL BL'
-        -> poEq (forwardF BL forward F rF d)
-               (forwardF BL' forward' F rF' d').
+        -> poEq (forwardF BL forward F rF d ST)
+               (forwardF BL' forward' F rF' d' ST).
 Proof.
-  intros d d' LE_d rF rF' LE_rf.
+  intros ST d d' LE_d rF rF' LE_rf.
   general induction F; inv LE_rf; simpl;
     try now (econstructor; simpl; eauto using @ann_R, @PIR2).
   split; [split|].
@@ -356,98 +303,34 @@ Proof.
     eapply IHF; eauto using get. eapply fwdMon; eauto using get.
 Qed.
 
-Lemma PIR2_zip_setTopAnnO X `{PartialOrder X} (A A':list (ann X)) (B B':list X)
-  : poLe A A'
-    -> poLe B B'
-    -> poLe ((@setTopAnn _) ⊜ A B) (@setTopAnn _ ⊜ A' B').
-Proof.
-  intros LE_A LE_B; simpl in *.
-  general induction LE_A; inv LE_B; simpl; eauto using PIR2.
-  - econstructor; eauto.
-    eauto using ann_R_setTopAnn.
-Qed.
-
-Lemma ann_poLe_joinTopAnn A `{JoinSemiLattice A} (a:A) (b:A) an bn
-  : poLe a b
-    -> ann_R poLe an bn
-    -> ann_R poLe (joinTopAnn an a) (joinTopAnn bn b).
-Proof.
-  intros.
-  inv H2; simpl; econstructor; try eapply join_struct; eauto.
-Qed.
-
-Lemma ann_poEq_joinTopAnn A `{JoinSemiLattice A} (a:A) (b:A) an bn
-  : poEq a b
-    -> ann_R poEq an bn
-    -> ann_R poEq (joinTopAnn an a) (joinTopAnn bn b).
-Proof.
-  intros.
-  inv H2; simpl; econstructor; eauto;
-    rewrite H1, H3; reflexivity.
-Qed.
-
-
-Lemma PIR2_zip_joinTopAnnO X `{JoinSemiLattice X} (A A':list (ann X)) (B B':list X)
-  : poLe A A'
-    -> poLe B B'
-    -> poLe ((@joinTopAnn _ _ _) ⊜ A B) (@joinTopAnn _ _ _ ⊜ A' B').
-Proof.
-  intros LE_A LE_B; simpl in *.
-  general induction LE_A; inv LE_B; simpl; eauto using PIR2.
-  - econstructor; eauto.
-    eauto using ann_poLe_joinTopAnn.
-Qed.
-
-Lemma PIR2_poEq_zip_setTopAnnO X `{PartialOrder X} (A A':list (ann X)) (B B':list X)
-  : poEq A A'
-    -> poEq B B'
-    -> poEq ((@setTopAnn _) ⊜ A B) (@setTopAnn _ ⊜ A' B').
-Proof.
-  intros LE_A LE_B; simpl in *.
-  general induction LE_A; inv LE_B; simpl; eauto using PIR2.
-  - econstructor; eauto.
-    eauto using ann_R_setTopAnn.
-Qed.
-
-Lemma PIR2_poEq_zip_joinTopAnnO X `{JoinSemiLattice X} (A A':list (ann X)) (B B':list X)
-  : poEq A A'
-    -> poEq B B'
-    -> poEq ((@joinTopAnn _ _ _) ⊜ A B) (@joinTopAnn _ _ _ ⊜ A' B').
-Proof.
-  intros LE_A LE_B; simpl in *.
-  general induction LE_A; inv LE_B; simpl; eauto using PIR2.
-  - econstructor; eauto.
-    eauto using ann_poEq_joinTopAnn.
-Qed.
-
-Lemma forward_monotone D `{JoinSemiLattice D}
-      (f: bool -> DomainSSA.Dom D -> exp -> ؟ D)
-      (fr : bool -> Dom D -> op -> bool * bool)
-      (fMon: forall e a a', a ⊑ a' -> forall b b', b ⊑ b' -> f b a e ⊑ f b' a' e)
-      (frMon:forall e a a',
-            a ⊑ a' -> forall b b', b ⊑ b' -> fr b a e ⊑ fr b' a' e)
-  : forall (s : stmt) (ZL:list params),
-    forall (d d' : Dom D), d ⊑ d'
+Lemma forward_monotone sT D `{JoinSemiLattice D}
+      (f: forall U : ⦃nat⦄, bool -> VDom U D -> exp -> ؟ D)
+      (fr: forall U : ⦃nat⦄, bool -> VDom U D -> op -> bool * bool)
+      (fMon: forall U e (a a':VDom U D), a ⊑ a' -> forall b b', b ⊑ b' -> f _ b a e ⊑ f _ b' a' e)
+      (frMon:forall U e (a a':VDom U D),
+            a ⊑ a' -> forall b b', b ⊑ b' -> fr _ b a e ⊑ fr _ b' a' e)
+  : forall (s : stmt) (ST:subTerm s sT) (ZL:list params) ZLIncl,
+    forall (d d' : VDom (occurVars sT) D), d ⊑ d'
       -> forall (r r':ann bool), r ⊑ r'
-      -> forward f fr ZL s d r ⊑ forward f fr ZL s d' r'.
+      -> forward f fr ZL ZLIncl ST d r ⊑ forward f fr ZL ZLIncl ST d' r'.
 Proof with eauto using poLe_setTopAnn, poLe_getAnni.
   intros s.
-  sind s; destruct s; intros ZL d d' LE_d r r'  LE_r;
+  sind s; destruct s; intros ST ZL ZLIncl d d' LE_d r r'  LE_r;
     destruct r; inv LE_r;
       simpl forward; repeat let_pair_case_eq; subst;
         eauto 10 using @ann_R;
         try now (econstructor; simpl; eauto using @ann_R).
-  - simpl. pose proof (fMon e  _ _ LE_d _ _ H3); eauto.
+  - unfold domupdd. simpl. pose proof (fMon _ e  _ _ LE_d _ _ H3); eauto.
     simpl in *. split; dcr; eauto; [split; eauto|]; simpl;
                   eauto 20 using domupd_le, ann_R_setTopAnn, ann_R.
     + eapply IH; eauto using domupd_le, ann_R_setTopAnn.
     + econstructor; eauto. eapply IH; eauto using domupd_le.
       eauto using ann_R_setTopAnn.
     + eapply IH; eauto using domupd_le, ann_R_setTopAnn.
-  - pose proof (fMon (Operation e) _ _ LE_d) as LE_f.
-    pose proof (frMon e _ _ LE_d) as LE_fr.
-    pose proof (IH s1 ltac:(eauto) ZL) as LE1; eauto.
-    pose proof (IH s2 ltac:(eauto) ZL) as LE2; eauto.
+  - pose proof (fMon _ (Operation e) _ _ LE_d) as LE_f.
+    pose proof (frMon _ e _ _ LE_d) as LE_fr.
+    pose proof (IH s1 ltac:(eauto) (subTerm_EQ_If1 eq_refl ST) ZL ZLIncl) as LE1; eauto.
+    pose proof (IH s2 ltac:(eauto) (subTerm_EQ_If2 eq_refl ST) ZL ZLIncl) as LE2; eauto.
     split; [split|];simpl.
     + eapply LE2; eauto. eapply LE1; eauto.
       eapply ann_R_setTopAnn; eauto. eapply LE_fr; eauto.
@@ -478,7 +361,8 @@ Proof with eauto using poLe_setTopAnn, poLe_getAnni.
    + pose proof (@update_at_poLe bool _ _ _ ZL l _ _ H2).
      simpl in *. eauto.
   - split; [split|]; simpl.
-    + eapply forwardF_monotone; eauto.
+    + pose proof (@forwardF_monotone sT (sTDom D) _); eauto.
+      eapply H1; eauto.
       eapply IH; eauto.
       eapply ann_R_setTopAnn; eauto.
       eapply PIR2_zip_joinTopAnnO; eauto.
@@ -492,7 +376,8 @@ Proof with eauto using poLe_setTopAnn, poLe_getAnni.
         eauto with len.
       * eapply get_PIR2.
         eapply (@PIR2_zip_setTopAnnO bool PartialOrder_bool).
-        eapply forwardF_monotone; eauto.
+        pose proof (@forwardF_monotone sT (sTDom D) _); eauto.
+        eapply H1; eauto.
         eapply IH; eauto.
         eapply ann_R_setTopAnn; eauto.
         eapply (@PIR2_zip_joinTopAnnO bool PartialOrder_bool); eauto.
@@ -524,34 +409,34 @@ Proof with eauto using poLe_setTopAnn, poLe_getAnni.
       eapply ann_R_setTopAnn; eauto.
 Qed.
 
-Lemma forward_ext D `{JoinSemiLattice D}
-      (f: bool -> DomainSSA.Dom D -> exp -> ؟ D)
-      (fr : bool -> Dom D -> op -> bool * bool)
-      (fMon: forall e a a', a ≣ a' -> forall b b', b ≣ b' -> f b a e ≣ f b' a' e)
-      (frMon:forall e a a',
-            a ≣ a' -> forall b b', b ≣ b' -> fr b a e ≣ fr b' a' e)
-  : forall (s : stmt) (ZL:list params),
-    forall (d d' : Dom D), d ≣ d'
+Lemma forward_ext sT D `{JoinSemiLattice D}
+      (f: forall U : ⦃nat⦄, bool -> VDom U D -> exp -> ؟ D)
+      (fr: forall U : ⦃nat⦄, bool -> VDom U D -> op -> bool * bool)
+      (fMon: forall U e (a a':VDom U D), a ≣ a' -> forall b b', b ≣ b' -> f _ b a e ≣ f _ b' a' e)
+      (frMon:forall U e (a a':VDom U D),
+            a ≣ a' -> forall b b', b ≣ b' -> fr _ b a e ≣ fr _ b' a' e)
+  : forall (s : stmt) (ST:subTerm s sT) (ZL:list params) ZLIncl,
+    forall (d d' : VDom (occurVars sT) D), d ≣ d'
       -> forall (r r':ann bool), r ≣ r'
-      -> forward f fr ZL s d r ≣ forward f fr ZL s d' r'.
+      -> forward f fr ZL ZLIncl ST d r ≣ forward f fr ZL ZLIncl ST d' r'.
 Proof with eauto using poLe_setTopAnn, poLe_getAnni.
   intros s.
-  sind s; destruct s; intros ZL d d' LE_d r r'  LE_r;
+  sind s; destruct s; intros ST ZL ZLIncl d d' LE_d r r'  LE_r;
     destruct r; inv LE_r;
       simpl forward; repeat let_pair_case_eq; subst;
         eauto 10 using @ann_R;
         try now (econstructor; simpl; eauto using @ann_R).
-  - simpl. pose proof (fMon e  _ _ LE_d _ _ H3); eauto.
+  - unfold domupdd. simpl. pose proof (fMon _ e  _ _ LE_d _ _ H3); eauto.
     simpl in *. split; dcr; eauto; [split; eauto|]; simpl;
                   eauto 20 using domupd_le, ann_R_setTopAnn, ann_R.
     + eapply IH; eauto using domupd_eq, ann_R_setTopAnn.
     + econstructor; eauto. eapply IH; eauto using domupd_eq.
       eauto using ann_R_setTopAnn.
     + eapply IH; eauto using domupd_eq, ann_R_setTopAnn.
-  - pose proof (fMon (Operation e) _ _ LE_d) as LE_f.
-    pose proof (frMon e _ _ LE_d) as LE_fr.
-    pose proof (IH s1 ltac:(eauto) ZL) as LE1; eauto.
-    pose proof (IH s2 ltac:(eauto) ZL) as LE2; eauto.
+  - pose proof (fMon _ (Operation e) _ _ LE_d) as LE_f.
+    pose proof (frMon _ e _ _ LE_d) as LE_fr.
+    pose proof (IH s1 ltac:(eauto) (subTerm_EQ_If1 eq_refl ST) ZL ZLIncl) as LE1; eauto.
+    pose proof (IH s2 ltac:(eauto) (subTerm_EQ_If2 eq_refl ST) ZL ZLIncl) as LE2; eauto.
     split; [split|];simpl.
     + eapply LE2; eauto. eapply LE1; eauto.
       eapply ann_R_setTopAnn; eauto. eapply LE_fr; eauto.
@@ -580,7 +465,8 @@ Proof with eauto using poLe_setTopAnn, poLe_getAnni.
    + econstructor; eauto.
    + inv H2. reflexivity.
   - split; [split|]; simpl.
-    + eapply forwardF_ext; eauto.
+    + pose proof (@forwardF_ext sT (sTDom D) _); eauto.
+      eapply H1; eauto.
       eapply IH; eauto.
       eapply ann_R_setTopAnn; eauto.
       eapply PIR2_poEq_zip_joinTopAnnO; eauto.
@@ -627,26 +513,27 @@ Proof with eauto using poLe_setTopAnn, poLe_getAnni.
 Qed.
 
 
-Lemma forwardF_PIR2  D `{JoinSemiLattice D} BL ZL
+Lemma forwardF_PIR2 sT D `{JoinSemiLattice D} BL ZL ZLIncl
       (F:list (params * stmt)) sa a (Len1:❬F❭ = ❬sa❭)
       (Len2:❬BL❭ = ❬ZL❭)
-      (f: bool -> DomainSSA.Dom D -> exp -> ؟ D)
-      (fr : bool -> Dom D -> op -> bool * bool)
-      (EQ: forall n Zs r, get F n Zs -> get sa n r ->
-                        poEq (fst (fst (forward f fr ZL (snd Zs) a r))) a)
-      (fExt: forall e a a', a ≣ a' -> forall b b', b ≣ b' -> f b a e ≣ f b' a' e)
-      (frExt:forall e a a',
-            a ≣ a' -> forall b b', b ≣ b' -> fr b a e ≣ fr b' a' e)
-      n r Zs (Getsa:get sa n r) (GetF:get F n Zs)
+      (f: forall U : ⦃nat⦄, bool -> VDom U D -> exp -> ؟ D)
+      (fr: forall U : ⦃nat⦄, bool -> VDom U D -> op -> bool * bool)
+      (EQ: forall n Zs r (ST:subTerm (snd Zs) sT), get F n Zs -> get sa n r ->
+                        poEq (fst (fst (forward f fr ZL ZLIncl ST a r))) a)
+      (fExt: forall U e (a a':VDom U D), a ≣ a' -> forall b b', b ≣ b' -> f _ b a e ≣ f _ b' a' e)
+      (frExt:forall U e (a a':VDom U D),
+            a ≣ a' -> forall b b', b ≣ b' -> fr _ b a e ≣ fr _ b' a' e)
+      n r Zs (ST:subTerm (snd Zs) sT) (Getsa:get sa n r) (GetF:get F n Zs) STF
 :
   PIR2 impb
-       (snd (forward f fr ZL (snd Zs) a r))
-       (snd (forwardF BL (forward f fr ZL) F sa a)).
+       (snd (forward f fr ZL ZLIncl ST a r))
+       (snd (@forwardF sT (sTDom D) BL (forward f fr ZL ZLIncl) F sa a STF)).
 Proof.
   general induction n; isabsurd; simpl.
   - eapply PIR2_impb_orb_right.
     + len_simpl; eauto. intros. eauto with len.
-    + reflexivity.
+    + assert (ST = (STF 0 Zs (getLB xl Zs))).
+      eapply subTerm_PI. subst. reflexivity.
   - inv Getsa; inv GetF. simpl.
     eapply PIR2_impb_orb_left; eauto with len.
     etransitivity; [| eapply IHn; eauto using get].
@@ -665,23 +552,18 @@ Qed.
 
 
 Require Import Take.
-
-Lemma forwardF_get  (sT:stmt) (Dom:stmt->Type) BL ZL
+Lemma forwardF_get  (sT:stmt) D `{JoinSemiLattice D} BL ZL
       (F:list (params * stmt)) rF a ZLIncl
-      (f : forall (sT : stmt) (ZL : 〔params〕) (s : stmt),
-          subTerm s sT ->
-          list_union (of_list ⊝ ZL) [<=] occurVars sT
-          -> Dom sT -> bool -> Dom sT)
-      fr
+      f fr
       (ST:forall n s, get F n s -> subTerm (snd s) sT) n aa
-           (GetBW:get (snd (fst (@forwardF Dom BL (@forward sT Dom f fr ZL ZLIncl) F rF a ST))) n aa)
+           (GetBW:get (snd (fst (@forwardF sT (sTDom D) BL (forward f fr ZL ZLIncl) F rF a ST))) n aa)
   :
     { Zs : params * stmt &
            {GetF : get F n Zs &
                    { r : ann bool &
                          {GetrF : get rF n r &
                                   { ST' : subTerm (snd Zs) sT &
-                                          { ST'' : forall (n0 : nat) (s : params * stmt), get (take n F) n0 s -> subTerm (snd s) sT | aa = snd (fst (forward Dom f fr ZL ZLIncl ST' (fst (fst (@forwardF sT Dom BL (@forward sT Dom f fr ZL ZLIncl) (take n F) (take n rF) a ST''))) r))
+                                          { ST'' : forall (n0 : nat) (s : params * stmt), get (take n F) n0 s -> subTerm (snd s) sT | aa = snd (fst (forward f fr ZL ZLIncl ST' (fst (fst (@forwardF sT (sTDom D) BL (forward f fr ZL ZLIncl) (take n F) (take n rF) a ST''))) r))
   } } } } } }.
 Proof.
   eapply get_getT in GetBW.
@@ -693,7 +575,7 @@ Proof.
     edestruct IHn as [Zs [? [? [? [? [? ]]]]]]; eauto; subst. simpl in *. subst.
     assert (STx:forall (n1 : nat) (s : params * stmt),
                get (p::take n F) n1 s -> subTerm (snd s) sT). {
-      intros. inv H; eauto using get.
+      intros. inv H1; eauto using get.
     }
     assert (STEQ1:(ST 0 p (getLB F p) = (STx 0 p (getLB (take n F) p))))
       by eapply subTerm_PI.
@@ -710,36 +592,19 @@ Qed.
 
 Require Import FiniteFixpointIteration.
 
-Instance LowerBounded_ann (s:stmt) A `{LowerBounded A}
-  : LowerBounded ({ a : ann bool | annotation s a }) :=
-  {
-    bottom := exist _ (setAnn bottom s) _
-  }.
-Proof.
-  - eapply setAnn_annotation.
-  - intros []. simpl.
-    general induction a; simpl; eauto using @ann_R.
-    + econstructor; eauto with len.
-      intros; inv_get. exploit H1; eauto.
-Defined.
 
-
-Lemma forward_annotation Dom sT s (ST:subTerm s sT)
-      (f:forall (sT : stmt) (ZL : 〔params〕) (s : stmt),
-          subTerm s sT ->
-          list_union (of_list ⊝ ZL) [<=] occurVars sT -> Dom sT -> bool -> Dom sT)
-      fr
-      ZL ZLIncl d r
+Lemma forward_annotation sT D `{JoinSemiLattice D} s (ST:subTerm s sT)
+      f fr ZL ZLIncl d r
       (AN:annotation s r)
-  : annotation s (snd (fst (forward Dom f fr ZL ZLIncl ST d r))).
+  : annotation s (snd (fst (forward f fr ZL ZLIncl ST d r))).
 Proof.
-  revert ST ZL ZLIncl d r AN.
+  revert ZL ZLIncl d r AN.
   sind s; intros; invt @annotation; simpl;
     repeat let_pair_case_eq; subst; simpl;
       eauto 20 using @annotation, setTopAnn_annotation.
   - econstructor; eauto 20 using setTopAnn_annotation.
     + len_simpl; try reflexivity.
-      rewrite H.
+      rewrite H1.
       rewrite !min_l; eauto with len.
       rewrite !min_l; eauto with len.
       rewrite !min_l; eauto with len.
@@ -747,35 +612,27 @@ Proof.
       eauto with len.
     + intros; inv_get.
       eapply setTopAnn_annotation; eauto.
-      eapply forwardF_get in H4. destruct H4; dcr; subst.
+      eapply forwardF_get in H6. destruct H6; dcr; subst.
       inv_get. eapply IH; eauto.
       eapply setTopAnn_annotation; eauto.
 Qed.
 
 
-Instance makeForwardAnalysis (Dom:stmt -> Type)
-         {PO:forall s, PartialOrder (Dom s)}
-         (BSL:forall s, JoinSemiLattice (Dom s))
-         (LB: forall s, @LowerBounded (Dom s) (PO s))
-         (f: forall (sT : stmt) (ZL : 〔params〕) (s : stmt),
-             subTerm s sT ->
-             list_union (of_list ⊝ ZL) [<=] occurVars sT -> Dom sT -> bool -> Dom sT)
-         (fr:forall (sT : stmt) (e : op),
-             Op.freeVars e [<=] occurVars sT -> Dom sT -> bool -> bool * bool)
-         (fMon:forall sT s (ST:subTerm s sT) ZL
-                 (ZLIncl:list_union (of_list ⊝ ZL) [<=] occurVars sT),
-             forall a b, a ⊑ b ->
-                    forall r r', r ⊑ r' ->
-                            f sT ZL s ST ZLIncl a r ⊑ f sT ZL s ST ZLIncl b r')
-         (frMon:forall sT e s (ST:subTerm s sT) FVIncl,
-          forall a a',
-            a ⊑ a' -> forall b b', b ⊑ b' -> fr sT e FVIncl a b ⊑ fr sT e FVIncl a' b')
-         (Trm: forall s, Terminating (Dom s) poLt)
+Instance makeForwardAnalysis D
+         {PO:PartialOrder D}
+         (BSL:JoinSemiLattice D)
+         (LB:LowerBounded D)
+         (f: forall U : ⦃nat⦄, bool -> VDom U D -> exp -> ؟ D)
+         (fr: forall U : ⦃nat⦄, bool -> VDom U D -> op -> bool * bool)
+         (fMon: forall U e (a a':VDom U D), a ⊑ a' -> forall b b', b ⊑ b' -> f _ b a e ⊑ f _ b' a' e)
+         (frMon:forall U e (a a':VDom U D),
+             a ⊑ a' -> forall b b', b ⊑ b' -> fr _ b a e ⊑ fr _ b' a' e)
+         (Trm: Terminating D poLt)
 
-  : forall s, Iteration (Dom s * { a : ann bool | annotation s a }) :=
+  : forall s, Iteration (VDom (occurVars s) D * { a : ann bool | annotation s a }) :=
   {
     step := fun dr =>
-             let a := forward Dom f fr nil (incl_empty _ (occurVars s)) (subTerm_refl s)
+             let a := forward f fr nil (incl_empty _ (occurVars s)) (subTerm_refl s)
                              (fst dr) (proj1_sig (snd dr)) in
              (fst (fst a), exist (fun a => annotation s a) (snd (fst a)) _);
     initial_value := bottom
@@ -785,49 +642,24 @@ Proof.
   - subst a.
     eapply forward_annotation; eauto.
     eapply (proj2_sig (snd dr)).
-  - eapply s.
   - eapply bottom_least.
   - eapply terminating_pair; eauto.
-    eapply terminating_sig; eauto.
-    eapply terminating_ann.
-    eapply terminating_bool.
+    + eapply terminating_Dom; eauto.
+    + eapply terminating_sig; eauto.
+      eapply terminating_ann.
+      eapply terminating_bool.
   - hnf; intros.
-    eapply (forward_monotone Dom f fr (fMon s) (frMon s)); eauto.
+    eapply (forward_monotone f fr fMon frMon); eauto.
     eapply H. eapply H.
 Defined.
 
-
-
-Lemma PIR2_setTopAnn_zip_left X (R:X->X->Prop) `{Reflexive _ R} (A:list (ann X)) B
-  : PIR2 R (Take.take ❬A❭ B) (getAnn ⊝ A)
-    -> PIR2 (ann_R R) (@setTopAnn _ ⊜ A B) A.
-Proof.
-  intros P. general induction P; destruct A, B; isabsurd; eauto using PIR2.
-  simpl in *. clear_trivial_eqs.
-  econstructor; eauto.
-  eapply ann_R_setTopAnn_left; eauto.
-Qed.
-
-Lemma PIR2_joinTopAnn_zip_left X `{JoinSemiLattice X} (A:list (ann X)) B
-  : PIR2 poLe (Take.take ❬A❭ B) (getAnn ⊝ A)
-    -> PIR2 poEq (@joinTopAnn _ _ _ ⊜ A B) A.
-Proof.
-  intros P. general induction P; destruct A,B; isabsurd; eauto using PIR2.
-  simpl in *. clear_trivial_eqs.
-  econstructor; eauto.
-  eapply ann_R_setTopAnn_left; eauto.
-  eapply poLe_antisymmetric. rewrite pf.
-  rewrite join_idempotent. eauto.
-  eapply join_poLe.
-Qed.
-
-Lemma snd_forwardF_inv Dom sT f fr BL ZL ZLIncl F sa AE STF
+Lemma snd_forwardF_inv (sT:stmt) D `{JoinSemiLattice D} f fr BL ZL ZLIncl F sa AE STF
       (P1:PIR2 (ann_R eq)
                (setTopAnn (A:=bool)
-                          ⊜ (snd (fst (forwardF BL (@forward sT Dom f fr ZL ZLIncl) F
+                          ⊜ (snd (fst (@forwardF sT (sTDom D) BL (forward f fr ZL ZLIncl) F
                                                 (joinTopAnn (A:=bool) ⊜ sa BL) AE STF)))
                           (snd (forwardF BL
-                                         (@forward _ _ f fr ZL ZLIncl) F
+                                         (forward f fr ZL ZLIncl) F
                                          (joinTopAnn (A:=bool) ⊜ sa BL) AE STF))) sa)
       (Len1:❬F❭ = ❬sa❭) (Len2:❬F❭ <= ❬BL❭) (Len3:❬ZL❭ = ❬BL❭)
   : PIR2 (ann_R eq) (joinTopAnn (A:=bool) ⊜ sa BL) sa.
@@ -835,19 +667,19 @@ Proof.
   eapply PIR2_ann_R_get in P1.
   rewrite getAnn_setTopAnn_zip in P1.
   pose proof (PIR2_joinTopAnn_zip_left sa BL).
-  eapply H; clear H.
+  eapply H1; clear H1.
   etransitivity.
   eapply PIR2_take.
-  eapply (@forwardF_mon sT _ f fr ZL ZLIncl BL ltac:(omega) F (joinTopAnn (A:=bool) ⊜ sa BL) AE STF).
+  eapply (@forwardF_mon sT D _ _ f fr ZL ZLIncl BL ltac:(omega) F STF (joinTopAnn (A:=bool) ⊜ sa BL) AE).
   etransitivity. Focus 2.
   eapply PIR2_R_impl; try eapply P1; eauto.
   assert (❬sa❭ = (Init.Nat.min
           ❬snd
              (fst
-                (forwardF BL (@forward _ _ f fr ZL ZLIncl) F
+                (forwardF BL (forward f fr ZL ZLIncl) F
                    (joinTopAnn (A:=bool) ⊜ sa BL) AE STF))❭
           ❬snd
-             (forwardF BL (@forward _ _ f fr ZL ZLIncl) F (joinTopAnn (A:=bool) ⊜ sa BL)
+             (forwardF BL (forward f fr ZL ZLIncl) F (joinTopAnn (A:=bool) ⊜ sa BL)
                        AE STF)❭)). {
     clear P1.
     rewrite forwardF_length.
@@ -856,24 +688,27 @@ Proof.
         rewrite Len1; rewrite min_l; omega.
     + intros; len_simpl; eauto.
   }
-  rewrite H. reflexivity.
+  rewrite H1. reflexivity.
 Qed.
 
-Lemma snd_forwardF_inv' Dom sT f fr BL ZL ZLIncl F sa AE STF
+Lemma snd_forwardF_inv' sT D `{JoinSemiLattice D}
+      (f: forall U : ⦃nat⦄, bool -> VDom U D -> exp -> ؟ D)
+      (fr: forall U : ⦃nat⦄, bool -> VDom U D -> op -> bool * bool)
+      BL ZL ZLIncl F sa AE STF
       (P1:PIR2 (ann_R eq)
                (setTopAnn (A:=bool)
-                          ⊜ (snd (fst (forwardF BL (@forward Dom sT f fr ZL ZLIncl) F
+                          ⊜ (snd (fst (forwardF BL (forward f fr ZL ZLIncl) F
                                                 (joinTopAnn (A:=bool) ⊜ sa BL) AE STF)))
                           (snd (forwardF BL
-                                         (@forward _ _ f fr ZL ZLIncl) F
+                                         (forward f fr ZL ZLIncl) F
                                          (joinTopAnn (A:=bool) ⊜ sa BL) AE STF))) sa)
       (Len1:❬F❭ = ❬sa❭) (Len2:❬F❭ <= ❬BL❭) (Len3:❬ZL❭ = ❬BL❭)
   : PIR2 (ann_R eq)
-              (snd (fst (forwardF BL (@forward Dom sT f fr ZL ZLIncl) F
-                                                (joinTopAnn (A:=bool) ⊜ sa BL) AE STF))) sa.
+              (snd (fst (@forwardF sT (sTDom D) BL (forward f fr ZL ZLIncl) F
+                                   (joinTopAnn (A:=bool) ⊜ sa BL) AE STF))) sa.
 Proof.
   assert (P2:PIR2 poLe (Take.take ❬sa❭
-                               (snd (forwardF BL (@forward _ _ f fr ZL ZLIncl) F
+                               (snd (forwardF BL (forward f fr ZL ZLIncl) F
                                               (joinTopAnn (A:=bool) ⊜ sa BL) AE
                                               STF))) (getAnn ⊝ sa)). {
     eapply PIR2_ann_R_get in P1.
@@ -883,10 +718,10 @@ Proof.
     assert (❬sa❭ = (Init.Nat.min
                       ❬snd
                          (fst
-                            (forwardF BL (@forward _ _ f fr ZL ZLIncl) F
+                            (forwardF BL (forward f fr ZL ZLIncl) F
                                       (joinTopAnn (A:=bool) ⊜ sa BL) AE STF))❭
                       ❬snd
-                         (forwardF BL (@forward _ _ f fr ZL ZLIncl) F (joinTopAnn (A:=bool) ⊜ sa BL)
+                         (forwardF BL (forward f fr ZL ZLIncl) F (joinTopAnn (A:=bool) ⊜ sa BL)
                                    AE STF)❭)). {
       clear P1.
       rewrite forwardF_length.
@@ -895,22 +730,22 @@ Proof.
           rewrite Len1; rewrite min_l; omega.
       + intros; len_simpl; eauto.
     }
-    rewrite H. reflexivity.
+    rewrite H1. reflexivity.
   }
   assert (PIR2 (ann_R eq) (joinTopAnn (A:=bool) ⊜ sa BL) sa). {
     pose proof (PIR2_joinTopAnn_zip_left sa BL).
-    eapply H; clear H.
+    eapply H1; clear H1.
     etransitivity.
     eapply PIR2_take.
-    eapply (@forwardF_mon Dom sT f fr ZL ZLIncl BL ltac:(omega) F (joinTopAnn (A:=bool) ⊜ sa BL) AE STF). eauto.
+    eapply (@forwardF_mon sT D _ _ f fr ZL ZLIncl BL ltac:(omega) F STF (joinTopAnn (A:=bool) ⊜ sa BL) AE). eauto.
   }
   etransitivity; try eapply P1.
   symmetry.
   eapply (PIR2_setTopAnn_zip_left); eauto.
   rewrite <- forwardF_mon';[|len_simpl; rewrite min_l; eauto; omega].
   - len_simpl. rewrite min_r, min_l; eauto; try rewrite Len1; try rewrite min_l; try omega.
-    eapply PIR2_ann_R_get in H.
-    rewrite H.
+    eapply PIR2_ann_R_get in H1.
+    rewrite H1.
     eapply PIR2_ann_R_get in P1.
     etransitivity; try eapply P1.
     eapply PIR2_get; intros; inv_get.
@@ -923,27 +758,20 @@ Qed.
 
 
 
-Lemma snd_forwardF_inv_get (Dom:stmt -> Type) sT `{PartialOrder (Dom sT)} f fr BL ZL ZLIncl F sa AE STF
+Lemma snd_forwardF_inv_get sT D `{JoinSemiLattice D} f fr BL ZL ZLIncl F sa AE STF
       (Len1:❬F❭ = ❬sa❭) (Len2:❬F❭ <= ❬BL❭) (Len3:❬ZL❭ = ❬BL❭)
       (P1:PIR2 (ann_R eq)
-               (snd (fst (forwardF BL (@forward sT Dom f fr ZL ZLIncl) F
+               (snd (fst (@forwardF sT (sTDom D)  BL (forward f fr ZL ZLIncl) F
                                   (joinTopAnn (A:=bool) ⊜ sa BL) AE STF))) sa)
       (P2:PIR2 (ann_R eq) (joinTopAnn (A:=bool) ⊜ sa BL) sa)
-      (EQ: forall n Zs r ST, get F n Zs -> get sa n r ->
-                        poEq (fst (fst (@forward sT Dom f fr ZL ZLIncl (snd Zs) ST AE r))) AE)
-      (fExt: forall (s : stmt) (ST0 : subTerm s sT) (ZL0 : 〔params〕)
-               (ZLIncl0 : list_union (of_list ⊝ ZL0) [<=] occurVars sT)
-               (a a' : Dom sT),
-          a ≣ a' ->
-          forall b b' : bool,
-            b ≣ b' -> f sT ZL0 s ST0 ZLIncl0 a b ≣ f sT ZL0 s ST0 ZLIncl0 a' b')
-      (frExt:  forall (e : op) (s : stmt),
-          subTerm s sT ->
-          forall (FVIncl : Op.freeVars e [<=] occurVars sT) (a a' : Dom sT),
-            a ≣ a' -> forall b b' : bool, b ≣ b' -> fr sT e FVIncl a b ≣ fr sT e FVIncl a' b')
+      (EQ: forall n Zs r (ST:subTerm (snd Zs) sT), get F n Zs -> get sa n r ->
+                        poEq (fst (fst (forward f fr ZL ZLIncl ST AE r))) AE)
+      (fExt: forall U e (a a':VDom U D), a ≣ a' -> forall b b', b ≣ b' -> f _ b a e ≣ f _ b' a' e)
+      (frExt:forall U e (a a':VDom U D),
+          a ≣ a' -> forall b b', b ≣ b' -> fr _ b a e ≣ fr _ b' a' e)
       n r Zs (Getsa:get sa n r)
-      (GetF:get F n Zs) STZs
-  : ann_R eq (snd (fst (@forward _ _ f fr ZL ZLIncl (snd Zs) STZs AE r))) r.
+      (GetF:get F n Zs) (STZs:subTerm (snd Zs) sT)
+  : ann_R eq (snd (fst (forward f fr ZL ZLIncl STZs AE r))) r.
 Proof.
   rewrite forwardF_ext in P1; try eapply P2; try reflexivity.
   Focus 2. intros. eapply forward_ext; eauto.
@@ -952,12 +780,13 @@ Proof.
   destruct BL; isabsurd; simpl in *. inv Getsa; inv GetF.
   - inv P1.
     assert((STF 0 Zs (@getLB (params * stmt) XL Zs)) = STZs).
-    eapply subTerm_PI. rewrite <- H0.
+    eapply subTerm_PI. rewrite <- H1.
     eapply pf.
   - inv P1.
     eapply IHLen1; eauto using get.
     Focus 2.
     rewrite forwardF_ext; eauto.
     intros. eapply forward_ext; eauto.
-    symmetry. eapply EQ; eauto using get. reflexivity. simpl. omega.
+    symmetry. eapply EQ; eauto using get. reflexivity.
+    simpl. omega.
 Qed.
