theories/IL/AnnotationLattice.v
@@ -1,0 +1,123 @@
+Require Import Util LengthEq Get Drop Map CSet MoreList DecSolve AllInRel.
+Require Import Var Val Exp Env IL OptionR.
+Require Import Infra.PartialOrder Terminating Infra.Lattice Annotation.
+
+Set Implicit Arguments.
+
+Lemma option_map_mon T `{PartialOrder T}  U `{PartialOrder U} (a a':option T) (f f': T -> U)
+  : a ⊑ a'
+    -> (forall x y, x ⊑ y -> f x ⊑ f' y)
+    -> option_map f a ⊑ option_map f' a'.
+Proof.
+  intros A; inv A; simpl;
+    clear_trivial_eqs; simpl; eauto using fstNoneOrR.
+Qed.
+
+
+Definition joinTopAnn A `{JoinSemiLattice A} (a:ann A) (b:A) :=
+  setTopAnn a (join (getAnn a) b).
+
+
+Lemma PIR2_zip_setTopAnnO X `{PartialOrder X} (A A':list (ann X)) (B B':list X)
+  : poLe A A'
+    -> poLe B B'
+    -> poLe ((@setTopAnn _) ⊜ A B) (@setTopAnn _ ⊜ A' B').
+Proof.
+  intros LE_A LE_B; simpl in *.
+  general induction LE_A; inv LE_B; simpl; eauto using PIR2.
+  - econstructor; eauto.
+    eauto using ann_R_setTopAnn.
+Qed.
+
+Lemma ann_poLe_joinTopAnn A `{JoinSemiLattice A} (a:A) (b:A) an bn
+  : poLe a b
+    -> ann_R poLe an bn
+    -> ann_R poLe (joinTopAnn an a) (joinTopAnn bn b).
+Proof.
+  intros.
+  inv H2; simpl; econstructor; try eapply join_struct; eauto.
+Qed.
+
+Lemma ann_poEq_joinTopAnn A `{JoinSemiLattice A} (a:A) (b:A) an bn
+  : poEq a b
+    -> ann_R poEq an bn
+    -> ann_R poEq (joinTopAnn an a) (joinTopAnn bn b).
+Proof.
+  intros.
+  inv H2; simpl; econstructor; eauto;
+    rewrite H1, H3; reflexivity.
+Qed.
+
+
+Lemma PIR2_zip_joinTopAnnO X `{JoinSemiLattice X} (A A':list (ann X)) (B B':list X)
+  : poLe A A'
+    -> poLe B B'
+    -> poLe ((@joinTopAnn _ _ _) ⊜ A B) (@joinTopAnn _ _ _ ⊜ A' B').
+Proof.
+  intros LE_A LE_B; simpl in *.
+  general induction LE_A; inv LE_B; simpl; eauto using PIR2.
+  - econstructor; eauto.
+    eauto using ann_poLe_joinTopAnn.
+Qed.
+
+Lemma PIR2_poEq_zip_setTopAnnO X `{PartialOrder X} (A A':list (ann X)) (B B':list X)
+  : poEq A A'
+    -> poEq B B'
+    -> poEq ((@setTopAnn _) ⊜ A B) (@setTopAnn _ ⊜ A' B').
+Proof.
+  intros LE_A LE_B; simpl in *.
+  general induction LE_A; inv LE_B; simpl; eauto using PIR2.
+  - econstructor; eauto.
+    eauto using ann_R_setTopAnn.
+Qed.
+
+Lemma PIR2_poEq_zip_joinTopAnnO X `{JoinSemiLattice X} (A A':list (ann X)) (B B':list X)
+  : poEq A A'
+    -> poEq B B'
+    -> poEq ((@joinTopAnn _ _ _) ⊜ A B) (@joinTopAnn _ _ _ ⊜ A' B').
+Proof.
+  intros LE_A LE_B; simpl in *.
+  general induction LE_A; inv LE_B; simpl; eauto using PIR2.
+  - econstructor; eauto.
+    eauto using ann_poEq_joinTopAnn.
+Qed.
+
+
+Instance LowerBounded_ann (s:stmt) A `{LowerBounded A}
+  : LowerBounded ({ a : ann bool | annotation s a }) :=
+  {
+    bottom := exist _ (setAnn bottom s) _
+  }.
+Proof.
+  - eapply setAnn_annotation.
+  - intros []. simpl.
+    general induction a; simpl; eauto using @ann_R.
+    + econstructor; eauto with len.
+      intros; inv_get. exploit H1; eauto.
+Defined.
+
+
+
+
+Lemma PIR2_setTopAnn_zip_left X (R:X->X->Prop) `{Reflexive _ R} (A:list (ann X)) B
+  : PIR2 R (Take.take ❬A❭ B) (getAnn ⊝ A)
+    -> PIR2 (ann_R R) (@setTopAnn _ ⊜ A B) A.
+Proof.
+  intros P. general induction P; destruct A, B; isabsurd; eauto using PIR2.
+  simpl in *. clear_trivial_eqs.
+  econstructor; eauto.
+  eapply ann_R_setTopAnn_left; eauto.
+Qed.
+
+Lemma PIR2_joinTopAnn_zip_left X `{JoinSemiLattice X} (A:list (ann X)) B
+  : PIR2 poLe (Take.take ❬A❭ B) (getAnn ⊝ A)
+    -> PIR2 poEq (@joinTopAnn _ _ _ ⊜ A B) A.
+Proof.
+  intros P. general induction P; destruct A,B; isabsurd; eauto using PIR2.
+  simpl in *. clear_trivial_eqs.
+  econstructor; eauto.
+  eapply ann_R_setTopAnn_left; eauto.
+  eapply poLe_antisymmetric. rewrite pf.
+  rewrite join_idempotent. eauto.
+  eapply join_poLe.
+Qed.
