theories/IL/Exp.v
@@ -1,5 +1,5 @@
-Require Import Util EqDec DecSolve Val CSet Map Env Option Get SetOperations Events.
-Require Export MoreList Op.
+Require Import Util EqDec DecSolve Val CSet Map Env Option Get SetOperations IL.Events.
+Require Export MoreList Isa.Op.
 
 Set Implicit Arguments.
 
